timeprot-use-f-kheap: Have get_(object|tcb), aobjs_of use f_kheap
Also a safety commit of partial fixes in AInvs. Next need to clarify how
and whether the object validity definitions in AInvs and the remaining
references to kheap in ASpec should change after all, and if so, how.

I converted in_user_frame (used only by store_word_offs) to use f_kheap
too, but the jury's still out on whether that's correct.

Signed-off-by: Robert Sison <robert.sison@unimelb.edu.au>

spec/abstract/KHeap_A.thy
@@ -52,14 +52,14 @@ lemma touch_object_def2:
 abbreviation ta_filter :: "machine_word set \<Rightarrow> kernel_object \<Rightarrow> obj_ref \<Rightarrow> kernel_object option" where
   "ta_filter ta obj ptr \<equiv> if obj_range ptr obj \<subseteq> ta then Some obj else None"
 
-abbreviation f_kheap :: "'z::state_ext state \<Rightarrow> obj_ref \<Rightarrow> kernel_object option" where
+definition f_kheap :: "'z::state_ext state \<Rightarrow> obj_ref \<Rightarrow> kernel_object option" where
   "f_kheap s \<equiv> kheap s |>> ta_filter (touched_addresses (machine_state s))"
 
 definition
   get_object :: "obj_ref \<Rightarrow> (kernel_object,'z::state_ext) s_monad"
 where
   "get_object ptr \<equiv> do
-     kh \<leftarrow> gets kheap;
+     kh \<leftarrow> gets f_kheap;
      assert (kh ptr \<noteq> None);
      return $ the $ kh ptr
    od"
@@ -73,20 +73,6 @@ where
      s \<leftarrow> get;
      put (s\<lparr>kheap := kheap s(ptr \<mapsto> obj)\<rparr>)
    od"
-
-text \<open>versions of @{term get_object} and @{term set_object} that obey the @{term touched_addresses}
-      pattern (for tracking cache stuff). This is temporary, for testing out
-      the effects of the new feature on a smaller scale.\<close>
-
-definition
-  get_object_x :: "obj_ref \<Rightarrow> (kernel_object,'z::state_ext) s_monad"
-where
-  "get_object_x ptr \<equiv> do
-     kh \<leftarrow> gets f_kheap;
-     assert (kh ptr \<noteq> None);
-     return $ the $ kh ptr
-   od"
-
 
 abbreviation
   ms_touched_addresses_update :: "(machine_word set \<Rightarrow> machine_word set) \<Rightarrow>
@@ -104,23 +90,13 @@ lemma simpler_do_machine_op_addTouchedAddresses_def:
   by (clarsimp simp: do_machine_op_def bind_def addTouchedAddresses_def simpler_gets_def
                         simpler_modify_def select_f_def return_def)
 
-definition
-  set_object_x :: "obj_ref \<Rightarrow> kernel_object \<Rightarrow> (unit,'z::state_ext) s_monad"
-where
-  "set_object_x ptr obj \<equiv> do
-     kobj <- get_object_x ptr;
-     assert (a_type kobj = a_type obj);
-     s \<leftarrow> get;
-     put (s\<lparr>kheap := kheap s(ptr \<mapsto> obj)\<rparr>)
-   od"
-
 section "TCBs"
 
 definition
   get_tcb :: "obj_ref \<Rightarrow> 'z::state_ext state \<Rightarrow> tcb option"
 where
   "get_tcb tcb_ref state \<equiv>
-   case kheap state tcb_ref of
+   case f_kheap state tcb_ref of
       None      \<Rightarrow> None
     | Some kobj \<Rightarrow> (case kobj of
         TCB tcb \<Rightarrow> Some tcb
